Good progress in proving EF statement

examples/Messaging/Toy.v
@@ -15,16 +15,17 @@ From Coinduction Require Import
 
 From CTree Require Import
      CTree
-     Interp
-     Interp.State
+     Interp.FoldStateT
      Interp.Log
      Interp.Network
-     Logic.Ltl
+     Logic.Ctl
      Misc.Vectors
      Eq
      SBisim.
 
-Import CTreeNotations VectorNotations LtlNotations Monads Log Network.
+From Equations Require Import Equations.
+
+Import CTreeNotations VectorNotations CtlNotations Monads Log Network.
 
 Local Open Scope fin_vector_scope.
 Local Open Scope ctree_scope.
@@ -41,31 +42,45 @@ Program Definition run{n C S} `{B1 -< C} `{B2 -< C} `{Bn -< C}
   
 Module Toy.
 
-  Notation heap := nat. 
   Notation Net := (Net 2 nat).
-  Notation State := (stateE heap).
+  Notation State := (stateE nat).
   Notation Sys := (vec 2 (ctree (Net +' State))).
 
   Section ParametricC.
     Context {C: Type -> Type} `{B0 -< C} `{B1 -< C} `{B2 -< C} `{Bn -< C}.
 
-    (*| This is a simple two process [a, b] system with a [nat] state.
-
-        For process (i in [a, b]) try to receive a number:
-        - If timeout without receiving, send current state [v] to the other process
-        - If [v] received, store [v] it and send [S v] to the other process 
+    (*| This is a simple two process  system called [echo/inc].
+        - Process [echo] sends its state [n]  and waits to hear back a new
+          number [m] from process [inc], stores [m] then repeats forever.
+        - Process [inc] waits to hear a number [n], then
+          sends back [S n], repeats forever.
     |*)
-    Definition example(them: uid 2): ctree (Net +' State) C void :=
+    Definition echo(them: uid 2): ctree (Net +' State) C void :=
+      daemon (
+          v <- get ;;
+          send them v ;;
+          CTree.iter (fun _ =>
+                        m <- recv ;;
+                        match m with
+                        | Some (Build_req id m) =>
+                            put m;;
+                            ret (inr tt)
+                        | None =>
+                            ret (inl tt)
+                        end) tt
+        ).
+
+    Definition inc: ctree (Net +' State) C void :=
       daemon (
           m <- recv ;;
           match m with
+          | Some (Build_req id m) =>
+              send id (S m);;
+              ret tt
           | None =>
-              v <- get ;;
-              send them v
-          | Some (Build_req _ v) =>
-              put v ;;
-              send them (S v)
-          end).
+              ret tt
+          end
+        ).
     
     Program Definition a : uid 2 := @of_nat_lt 0 2 _.
     Program Definition b : uid 2 := @of_nat_lt 1 2 _.
@@ -79,14 +94,84 @@ Module Toy.
     Variant is_eq: nat -> label (frameE 2 +' logE nat) -> Prop :=
       | IsEqualTo: forall n, is_eq n (obs (inr1 (Log n)) tt).
 
-    Lemma liveness: forall i,
-        let sys := run [example b; example a]%vector 0 in
-        sys |= InfinitelyOften (Spec (is_in_frame i)) -> (* Axiomatize fairness *)
-        sys |= Eventually (Spec (is_eq 2)).             (* Process [i] will count to 2 *)
+    (** Pick the nth branch *)
+    Ltac take_branch n :=
+      match goal with
+      | [ |- Logic.ex (fun l => Logic.ex (fun t =>  hrel_of (trans l) (brS (branchn ?m) ?k) t /\ _)) ] => exists tau, (k (n: fin m))
+      end.
+
+    Ltac take_enter :=
+      match goal with
+      | [ |- Logic.ex (fun l' => Logic.ex (fun t' => hrel_of (trans l') (enter ?i ;; ?k) _ /\ _)) ] => exists (obs (subevent _ (Enter i)) tt), k
+      end.
+    
+    Lemma eventually_counts: forall l,
+        let sys := run [echo b; inc]%vector 0 in
+        sys, l |= EF (lift (is_eq 1)).      (* Will count to [1] *)
     Proof.
-      intros i sys Fair.
-      (* WIP *)
+      intros l sys.
+      unfold sys, echo, inc, run, run_network, run_state_log in *.
+      clear sys.
+      cbn.
+      rewrite unfold_schedule.
+      rewrite bind_branch.
+      cbn.
+      (* Step the [EF] *)
+      rewrite ctl_ef_ex; right; unfold ex.
+      (* Take the branch [F1],  *)
+      take_branch b; split; [econstructor; reflexivity|].
+      simp schedule_one.
+      simp vector_replace; simpl.
+      (* Step the [EF] *)
+      rewrite ctl_ef_ex; right; unfold ex;
+        do 2 eexists; split; [eapply trans_trigger|].
+      (* Step the [EF] *)
+      rewrite ctl_ef_ex; right; unfold ex.
+      cbn.
+      exists tau; eexists; split.
+      eapply trans_guard.
+      simp vector_replace; simpl.
+      (* schedule *)
+      rewrite unfold_schedule; cbn.
+      apply trans_bind_l; [intro HV; inv HV |].
+      eapply trans_brS.
+      (* Better way to instantiate using Ltac ? *)
+      instantiate (1 := a).
+      rewrite bind_ret_l.
+      (* Step the [EF] *)
+      rewrite ctl_ef_ex; right; unfold ex;
+        do 2 eexists; split; [eapply trans_trigger|].
+      (* Step the [EF] *)
+      rewrite ctl_ef_ex; right; unfold ex.
+      exists tau; eexists.
+      simp schedule_one; cbn.
+      simp vector_replace; simpl; split.
+      eapply trans_guard.
+      (* Schedule  *)
+      rewrite unfold_schedule; cbn.
+      apply trans_bind_l; [intro HV; inv HV |].
+      eapply trans_brS.
+      rewrite bind_ret_l.
+      fold_subst.
+     
+      (* Semi Automated!! *)
+      (* Step the [EF] and schedule [a] *)
+      instantiate (1:=a);
+      rewrite ctl_ef_ex; right; unfold ex;
+        do 2 eexists; split; [eapply trans_trigger|];
+        rewrite ctl_ef_ex; right; unfold ex;
+        exists tau; eexists;
+        simp schedule_one; cbn; simp vector_replace; split; cbn;
+      (* For solving the [trans] *)
+        [eapply trans_guard; rewrite unfold_schedule; cbn;
+         eapply trans_bind_l; [intro HV; inv HV|];
+         eapply trans_brS; rewrite bind_ret_l
+        | rewrite bind_ret_l; fold_subst].
+      (* Now continuing...  *)
+      (* Ah I forgot which process to schedule now... *)
+      instantiate (1:= b). (* ? *)
     Admitted.
+
   End ParametricC.
 End Toy.
 
